Restored the proof somewhat

doc/formalization/Catala.Translation.fst
@@ -21,22 +21,17 @@ let translate_lit (l: D.lit) : Tot L.lit = match l with
   | D.LConflictError -> L.LError L.ConflictError
 
 let process_exceptions_f (tau: L.ty) : Tot L.exp =
-  let a = 0 in
-  let e = 1 in
-  let e' = 2 in
-  let a' = 3 in
-  let e'' = 4 in
-  L.EAbs (L.Named a) (L.TOption tau) (L.EAbs (L.Named e) (L.TArrow L.TUnit tau) (
-    L.EApp (L.EAbs (L.Named e') (L.TOption tau) (
-      L.EMatchOption (L.EVar a) tau
-        (L.EVar e')
-        (L.EAbs (L.Named a') tau (
-          L.EMatchOption (L.EVar e') tau
-            (L.EVar a)
-            (L.EAbs (L.Named e'') tau (L.ELit (L.LError L.ConflictError)))
+  L.EAbs (L.TOption tau) (L.EAbs (L.TArrow L.TUnit tau) (
+    L.EApp (L.EAbs (L.TOption tau) (
+      L.EMatchOption (L.EVar 2) tau
+        (L.EVar 0)
+        (L.EAbs tau (
+          L.EMatchOption (L.EVar 1) tau
+            (L.EVar 3)
+            (L.EAbs tau (L.ELit (L.LError L.ConflictError)))
         ))
     ))
-    (L.ECatchEmptyError (L.ESome (L.EApp (L.EVar e) (L.ELit L.LUnit) L.TUnit)) L.ENone)
+    (L.ECatchEmptyError (L.ESome (L.EApp (L.EVar 0) (L.ELit L.LUnit) L.TUnit)) L.ENone)
     (L.TOption tau)
   ))
 
@@ -65,13 +60,13 @@ let build_default_translation
     (L.EIf
       just cons
       (L.ELit (L.LError L.EmptyError)))
-    (L.EAbs (L.Named 0) tau (L.EVar 0))
+    (L.EAbs tau (L.EVar 0))
 
 let rec translate_exp (e: D.exp) : Tot L.exp = match e with
   | D.EVar x -> L.EVar x
   | D.EApp e1 e2 tau_arg ->
     L.EApp (translate_exp e1) (translate_exp e2) (translate_ty tau_arg)
-  | D.EAbs x ty body -> L.EAbs (L.Named x) (translate_ty ty) (translate_exp body)
+  | D.EAbs ty body -> L.EAbs (translate_ty ty) (translate_exp body)
   | D.ELit l -> L.ELit (translate_lit l)
   | D.EIf e1 e2 e3 -> L.EIf
     (translate_exp e1)
@@ -87,25 +82,25 @@ let rec translate_exp (e: D.exp) : Tot L.exp = match e with
 and translate_exp_list (l: list D.exp) : Tot (list L.exp) =
   match l with
   | [] -> []
-  | hd::tl -> (L.EAbs L.Silent L.TUnit (translate_exp hd))::(translate_exp_list tl)
+  | hd::tl -> (L.EAbs L.TUnit (L.subst L.increment (translate_exp hd)))::(translate_exp_list tl)
 
 let translate_env (g: D.env) : Tot L.env =
- FunctionalExtensionality.on_dom L.var_name
+ FunctionalExtensionality.on_dom L.var
    (fun v -> match g v with None -> None | Some t -> Some (translate_ty t))
 
 (*** Typing preservation *)
 
 (**** Helpers and lemmas *)
 
-let extend_translate_commute (g: D.env) (x: D.var) (tau: D.ty)
-    : Lemma (L.extend (translate_env g) x (translate_ty tau) == translate_env (D.extend g x tau))
+let extend_translate_commute (g: D.env) (tau: D.ty)
+    : Lemma (L.extend (translate_env g) (translate_ty tau) == translate_env (D.extend g tau))
   =
-  FunctionalExtensionality.extensionality L.var_name (fun _ -> option L.ty)
-    (L.extend (translate_env g) x (translate_ty tau))
-    (translate_env (D.extend g x tau))
+  FunctionalExtensionality.extensionality L.var (fun _ -> option L.ty)
+    (L.extend (translate_env g) (translate_ty tau))
+    (translate_env (D.extend g tau))
 
 let translate_empty_is_empty () : Lemma (translate_env D.empty == L.empty) =
-  FunctionalExtensionality.extensionality L.var_name (fun _ -> option L.ty)
+  FunctionalExtensionality.extensionality L.var (fun _ -> option L.ty)
     (translate_env D.empty)
     L.empty
 
@@ -142,12 +137,12 @@ let rec translation_preserves_typ (g: D.env) (e: D.exp) (tau: D.ty) : Lemma
   | D.EApp e1 e2 tau_arg ->
     translation_preserves_typ g e1 (D.TArrow tau_arg tau);
     translation_preserves_typ g e2 tau_arg
-  | D.EAbs x tau_arg body -> begin
+  | D.EAbs tau_arg body -> begin
     match tau with
     | D.TArrow tau_in tau_out ->
       if tau_in = tau_arg then begin
-        translation_preserves_typ (D.extend g x tau_in) body tau_out;
-        extend_translate_commute g x tau_in
+        translation_preserves_typ (D.extend g tau_in) body tau_out;
+        extend_translate_commute g tau_in
       end else ()
     | _ -> ()
   end
@@ -173,7 +168,7 @@ let rec translation_preserves_typ (g: D.env) (e: D.exp) (tau: D.ty) : Lemma
           (translate_exp just)
           (translate_exp cons)
           (L.ELit (L.LError L.EmptyError)))
-        (L.EAbs (L.Named 0) tau' (L.EVar 0))
+        (L.EAbs tau' (L.EVar 0))
       in
       let open FStar.Tactics in
       assert(L.typing (translate_env g) result_exp tau') by begin
@@ -206,7 +201,9 @@ and translation_preserves_typ_exceptions
     let thunked_tau' = L.TArrow L.TUnit tau' in
     assert(L.typing_list g' tl' thunked_tau');
     assert(L.typing g' hd' tau');
-    assert(L.typing g' (L.EAbs L.Silent L.TUnit hd') thunked_tau')
+    assert(L.typing g' hd' tau');
+    L.substitution_preserves_typing g' hd' tau' L.increment (L.extend g' L.TUnit) (fun x -> ());
+    assert(L.typing g' (L.EAbs L.TUnit (L.subst L.increment hd')) thunked_tau')
 #pop-options
 
 let translation_preserves_empty_typ (e: D.exp) (tau: D.ty) : Lemma
@@ -283,7 +280,7 @@ let rec l_values_dont_step (e: L.exp) : Lemma
     (decreases %[e; 1])
   =
   match e with
-  | L.EAbs _ _ _ -> ()
+  | L.EAbs _ _ -> ()
   | L.ELit _ -> ()
   | L.ENone -> ()
   | L.EList [] -> ()
@@ -329,47 +326,161 @@ let rec lift_multiple_l_steps
 
 
 #push-options "--fuel 9 --ifuel 0"
-let process_exceptions_untouched_by_subst (x: L.var_name) (e: L.exp) (tau: L.ty) : Lemma
-    (L.subst x e (process_exceptions_f tau) == process_exceptions_f tau)
+let process_exceptions_untouched_by_subst (s: L.var_to_exp) (tau: L.ty) : Lemma
+    (L.subst s (process_exceptions_f tau) == process_exceptions_f tau)
   =
   ()
 #pop-options
 
+let translate_var_to_exp (s: D.var_to_exp) : Tot L.var_to_exp = fun x -> translate_exp (s x)
+
+let double_increment : L.var_to_exp = fun y -> L.EVar (y + 2)
+
+let subst_abs_increment (x: L.var) =
+  if x = 0 then L.EVar 0 else L.EVar (x + 1)
+
+let dual_substitution_commutation_weakened
+  (s : L.var_to_exp{s 0 == L.EVar 0})
+  (e: L.exp)
+    : Lemma (L.subst subst_abs_increment (L.subst s e) ==
+      L.subst (L.subst_abs s) (L.subst subst_abs_increment e))
+  =
+  admit() // TODO
+
+let substitution_commutation_bonanza
+  (s: L.var_to_exp)
+  (e: L.exp)
+    : Lemma (L.subst (L.subst_abs L.increment) (L.subst (L.subst_abs s) e) ==
+      L.subst (L.subst_abs (L.subst_abs s)) (L.subst (L.subst_abs L.increment) e))
+  =
+  let aux (x: L.var) : Lemma ((L.subst_abs L.increment) x == subst_abs_increment x) = () in
+  Classical.forall_intro aux;
+  dual_substitution_commutation_weakened (L.subst_abs s) e
+
+#push-options "--fuel 3 --ifuel 1 --z3rlimit 40"
+let rec substitution_correctness_for_exception_thunking
+  (s: L.var_to_exp)
+  (e: L.exp)
+    : Lemma (
+      (L.EAbs L.TUnit (L.subst L.increment (L.subst s e))) ==
+      (L.subst s (L.EAbs L.TUnit (L.subst L.increment e)))
+    )
+  =
+  match e with
+  | L.EVar _ -> ()
+  | L.EAbs t body ->
+    // Top to down
+    assert(L.subst s e == L.EAbs t (L.subst (L.subst_abs s) body));
+    assert(L.subst L.increment (L.subst s e) ==
+      L.EAbs t (L.subst (L.subst_abs L.increment) (L.subst (L.subst_abs s) body)));
+    assert(L.EAbs L.TUnit (L.subst L.increment (L.subst s e)) ==
+      L.EAbs L.TUnit
+        (L.EAbs t (L.subst (L.subst_abs L.increment) (L.subst (L.subst_abs s) body))));
+    // Down to top
+    assert(L.subst L.increment e == L.EAbs t (L.subst (L.subst_abs L.increment) body));
+    assert(L.EAbs L.TUnit (L.subst L.increment e) ==
+      L.EAbs L.TUnit (L.EAbs t (L.subst (L.subst_abs L.increment) body)));
+    assert(L.subst s (L.EAbs L.TUnit (L.subst L.increment e)) ==
+      L.EAbs L.TUnit
+        (L.subst (L.subst_abs s) (L.EAbs t (L.subst (L.subst_abs L.increment) body))));
+    assert(L.subst s (L.EAbs L.TUnit (L.subst L.increment e)) ==
+      L.EAbs L.TUnit
+        (L.EAbs t
+          (L.subst (L.subst_abs (L.subst_abs s)) (L.subst (L.subst_abs L.increment) body))));
+    substitution_commutation_bonanza s body
+  | L.EApp e1 e2 _ ->
+    substitution_correctness_for_exception_thunking s e1;
+    substitution_correctness_for_exception_thunking s e2
+  | L.ELit _ -> ()
+  | L.EIf e1 e2 e3 ->
+    substitution_correctness_for_exception_thunking s e1;
+    substitution_correctness_for_exception_thunking s e2;
+    substitution_correctness_for_exception_thunking s e3
+  | L.ESome e1 -> substitution_correctness_for_exception_thunking s e1
+  | L.ENone -> ()
+  | L.EMatchOption e1 _ e2 e3 ->
+    substitution_correctness_for_exception_thunking s e1;
+    substitution_correctness_for_exception_thunking s e2;
+    substitution_correctness_for_exception_thunking s e3
+  | L.ECatchEmptyError e1 e2 ->
+    substitution_correctness_for_exception_thunking s e1;
+    substitution_correctness_for_exception_thunking s e2
+  | L.EFoldLeft e1 e2 _ e3 _ ->
+    substitution_correctness_for_exception_thunking s e1;
+    substitution_correctness_for_exception_thunking s e2;
+    substitution_correctness_for_exception_thunking s e3
+  | L.EList l ->
+    substitution_correctness_for_exception_thunking_list s l
+and substitution_correctness_for_exception_thunking_list
+  (s: L.var_to_exp)
+  (l: list L.exp)
+    : Lemma (
+      (L.EAbs L.TUnit (L.subst L.increment (L.subst s (L.EList l)))) ==
+      (L.subst s (L.EAbs L.TUnit (L.subst L.increment (L.EList l))))
+    )
+  =
+  match l with
+  | [] -> ()
+  | hd::tl ->
+    substitution_correctness_for_exception_thunking s hd;
+    substitution_correctness_for_exception_thunking_list s tl
+#pop-options
+
 #push-options "--fuel 3 --ifuel 1 --z3rlimit 50"
-let rec substitution_correctness (x: D.var) (e_x e: D.exp)
+let rec substitution_correctness (s: D.var_to_exp) (e: D.exp)
     : Lemma (ensures (
-      translate_exp (D.subst x e_x e) == L.subst x (translate_exp e_x) (translate_exp e)))
-      (decreases %[e; 1])
+      translate_exp (D.subst s e) ==
+        L.subst (translate_var_to_exp s) (translate_exp e)))
+      (decreases %[D.is_var_size e; D.is_renaming_size s; 1; e])
   =
   match e with
   | D.EVar y -> ()
   | D.ELit _ -> ()
   | D.EIf e1 e2 e3 ->
-    substitution_correctness x e_x e1;
-    substitution_correctness x e_x e2;
-    substitution_correctness x e_x e3
-  | D.EAbs _ _ body ->
-    substitution_correctness x e_x body
+    substitution_correctness s e1;
+    substitution_correctness s e2;
+    substitution_correctness s e3
+  | D.EAbs _ body ->
+    substitution_correctness (D.subst_abs s) body;
+    translate_var_to_exp_abs_commute s
   | D.EApp e1 e2 _ ->
-    substitution_correctness x e_x e1;
-    substitution_correctness x e_x e2
+    substitution_correctness s e1;
+    substitution_correctness s e2
   | D.EDefault exceptions just cons tau ->
-    substitution_correctness x e_x just;
-    substitution_correctness x e_x cons;
-    substitution_correctness_list x e_x e exceptions;
-    process_exceptions_untouched_by_subst x (translate_exp e_x) (translate_ty tau)
-and substitution_correctness_list (x: D.var) (e_x: D.exp) (e: D.exp) (l: list D.exp{l << e})
+    substitution_correctness s just;
+    substitution_correctness s cons;
+    substitution_correctness_list s exceptions;
+    process_exceptions_untouched_by_subst (translate_var_to_exp s) (translate_ty tau)
+and substitution_correctness_list (s: D.var_to_exp) (l: list D.exp)
     : Lemma (ensures (
-      translate_exp_list (D.subst_list x e_x l) ==
-      L.subst_list x (translate_exp e_x) (translate_exp_list l)))
-      (decreases %[e; 0; l])
+      translate_exp_list (D.subst_list s l) ==
+      L.subst_list (translate_var_to_exp s) (translate_exp_list l)))
+      (decreases %[1; D.is_renaming_size s; 1; l])
  =
  match l with
  | [] -> ()
  | hd::tl ->
-   substitution_correctness x e_x hd;
-   substitution_correctness_list x e_x e tl
+   let s' = translate_var_to_exp s in
+   substitution_correctness_list s tl;
+   substitution_correctness s hd;
+   substitution_correctness_for_exception_thunking s' (translate_exp hd)
+and translate_var_to_exp_abs_commute (s: D.var_to_exp)
+    : Lemma
+      (ensures (
+        FunctionalExtensionality.feq
+          (translate_var_to_exp (D.subst_abs s))
+          (L.subst_abs (translate_var_to_exp s))))
+      (decreases %[1; D.is_renaming_size s; 0])
+  =
+  let s1 = translate_var_to_exp (D.subst_abs s) in
+  let s2 = L.subst_abs (translate_var_to_exp s) in
+  let aux (x: L.var) : Lemma (s1 x == s2 x) =
+    if x = 0 then () else
+      substitution_correctness D.increment (s (x - 1))
+  in
+  Classical.forall_intro aux
 #pop-options
+
 
 let exceptions_smaller'
   (e: D.exp{match e with D.EDefault _ _ _ _ -> True | _ -> False})
@@ -529,23 +640,20 @@ let exceptions_head_lift'
   (cons: (typed_l_exp tau))
   : stepping_context tau tau
   =
-  let e' = 2 in
-  let a' = 3 in
-  let e'' = 4 in
   fun (hd: typed_l_exp tau) ->
     typ_process_exceptions_f L.empty tau;
-    L.typing_empty_can_be_extended acc (L.TOption tau) e' (L.TOption tau);
+    L.typing_empty_can_be_extended acc (L.TOption tau) (L.TOption tau);
     L.EMatchOption
     (L.EFoldLeft
       (process_exceptions_f tau)
       (L.EApp
-        (L.EAbs (L.Named e') (L.TOption tau) (
+        (L.EAbs (L.TOption tau) (
           L.EMatchOption acc tau
-            (L.EVar e')
-            (L.EAbs (L.Named a') tau (
-              L.EMatchOption (L.EVar e') tau
+            (L.EVar 0)
+            (L.EAbs tau (
+              L.EMatchOption (L.EVar 1) tau
                 L.ENone
-                (L.EAbs (L.Named e'') tau (L.ELit (L.LError L.ConflictError)))
+                (L.EAbs tau (L.ELit (L.LError L.ConflictError)))
             ))
          ))
          (L.ECatchEmptyError
@@ -558,7 +666,7 @@ let exceptions_head_lift'
     (L.EIf
       just cons
       (L.ELit (L.LError L.EmptyError)))
-    (L.EAbs (L.Named 0) tau (L.EVar 0))
+    (L.EAbs tau (L.EVar 0))
 #pop-options
 
 let exceptions_head_lift_is_stepping_agnostic
@@ -608,7 +716,7 @@ let exceptions_init_lift'
     (L.EIf
       just cons
       (L.ELit (L.LError L.EmptyError)))
-    (L.EAbs (L.Named 0) tau (L.EVar 0))
+    (L.EAbs tau (L.EVar 0))
 #pop-options
 
 let exceptions_init_lift_is_stepping_agnostic
@@ -647,9 +755,11 @@ let process_exceptions_applied
     : Tot (typed_l_exp (L.TOption tau))
   =
   typ_process_exceptions_f L.empty tau;
+  L.typing_empty_can_be_extended hd tau L.TUnit;
   L.EApp
-    (L.EApp (process_exceptions_f tau) acc (L.TOption tau))
-    (L.EAbs L.Silent L.TUnit hd) (L.TArrow L.TUnit tau)
+   (L.EApp (process_exceptions_f tau) acc (L.TOption tau))
+   (L.EAbs L.TUnit hd) (L.TArrow L.TUnit tau)
+
 
 #push-options "--fuel 7 --ifuel 2"
 let process_exceptions_applied_stepped
@@ -661,10 +771,10 @@ let process_exceptions_applied_stepped
   let e' = 2 in
   let a' = 3 in
   let e'' = 4 in
-  L.typing_empty_can_be_extended acc (L.TOption tau) e' (L.TOption tau);
-  L.EApp (L.EAbs (L.Named e') (L.TOption tau) (
-    L.EMatchOption acc tau (L.EVar e') (L.EAbs (L.Named a') tau (
-      L.EMatchOption (L.EVar e') tau L.ENone (L.EAbs (L.Named e'') tau
+  L.typing_empty_can_be_extended acc (L.TOption tau) (L.TOption tau);
+  L.EApp (L.EAbs (L.TOption tau) (
+    L.EMatchOption acc tau (L.EVar 0) (L.EAbs tau (
+      L.EMatchOption (L.EVar 1) tau L.ENone (L.EAbs  tau
         (L.ELit (L.LError L.ConflictError))
       )
     ))))
@@ -685,39 +795,40 @@ let process_exceptions_applied_stepping
   let e'' = 4 in
   let e1 : L.exp =
     L.EApp
-      (L.EAbs (L.Named e) (L.TArrow L.TUnit tau) (
-    L.EApp (L.EAbs (L.Named e') (L.TOption tau) (
+      (L.EAbs (L.TArrow L.TUnit tau) (
+    L.EApp (L.EAbs (L.TOption tau) (
       L.EMatchOption acc tau
-        (L.EVar e')
-        (L.EAbs (L.Named a') tau (
-          L.EMatchOption (L.EVar e') tau
+        (L.EVar 0)
+        (L.EAbs  tau (
+          L.EMatchOption (L.EVar 1) tau
             acc
-            (L.EAbs (L.Named e'') tau (L.ELit (L.LError L.ConflictError)))
+            (L.EAbs tau (L.ELit (L.LError L.ConflictError)))
         ))
     ))
     (L.ECatchEmptyError (L.ESome (L.EApp (L.EVar e) (L.ELit L.LUnit) L.TUnit)) L.ENone)
     (L.TOption tau)
   )
       )
-      (L.EAbs L.Silent L.TUnit hd) (L.TArrow L.TUnit tau)
+      (L.EAbs L.TUnit hd) (L.TArrow L.TUnit tau)
   in
   let e2 =
-    L.EApp (L.EAbs (L.Named e') (L.TOption tau) (
+    L.EApp (L.EAbs (L.TOption tau) (
       L.EMatchOption acc tau
-        (L.EVar e')
-        (L.EAbs (L.Named a') tau (
-          L.EMatchOption (L.EVar e') tau
+        (L.EVar 0)
+        (L.EAbs tau (
+          L.EMatchOption (L.EVar 1) tau
             acc
-            (L.EAbs (L.Named e'') tau (L.ELit (L.LError L.ConflictError)))
+            (L.EAbs tau (L.ELit (L.LError L.ConflictError)))
         ))
     ))
-    (L.ECatchEmptyError (L.ESome (L.EApp (L.EAbs L.Silent L.TUnit hd) (L.ELit L.LUnit) L.TUnit)) L.ENone)
+    (L.ECatchEmptyError (L.ESome (L.EApp (L.EAbs L.TUnit hd) (L.ELit L.LUnit) L.TUnit)) L.ENone)
     (L.TOption tau)
 
   in
-  assert(L.step (process_exceptions_applied tau acc hd) == Some e1);
+  assume(L.step (process_exceptions_applied tau acc hd) == Some e1);
   assume(L.step e1 == Some e2);
   admit()
+#pop-options
 
 #push-options "--fuel 7 --ifuel 2 --z3rlimit 50"
 let lift_multiple_l_steps_exceptions_head
@@ -732,20 +843,22 @@ let lift_multiple_l_steps_exceptions_head
     : Lemma
       (requires (take_l_steps tau hd n_hd == Some final_hd /\ L.is_value acc))
       (ensures (
+        L.typing_empty_can_be_extended hd tau L.TUnit;
         build_default_translation_typing
-          ((L.EAbs L.Silent L.TUnit hd)::tl) acc just cons tau L.empty;
+          ((L.EAbs L.TUnit hd)::tl) acc just cons tau L.empty;
         take_l_steps tau
-          (build_default_translation ((L.EAbs L.Silent L.TUnit hd)::tl) acc just cons tau)
+          (build_default_translation ((L.EAbs L.TUnit hd)::tl) acc just cons tau)
           (n_hd + 4) ==
             Some (exceptions_head_lift tau tl acc just cons final_hd)))
   =
-  build_default_translation_typing ((L.EAbs L.Silent L.TUnit hd)::tl) acc just cons tau L.empty;
+  L.typing_empty_can_be_extended hd tau L.TUnit;
+  build_default_translation_typing ((L.EAbs L.TUnit hd)::tl) acc just cons tau L.empty;
   let e' = 2 in
   let a' = 3 in
   let e'' = 4 in
-  let init_stepped = L.EApp (L.EAbs (L.Named e') (L.TOption tau) (
-    L.EMatchOption acc tau (L.EVar e') (L.EAbs (L.Named a') tau (
-      L.EMatchOption (L.EVar e') tau L.ENone (L.EAbs (L.Named e'') tau
+  let init_stepped = L.EApp (L.EAbs (L.TOption tau) (
+    L.EMatchOption acc tau (L.EVar 0) (L.EAbs tau (
+      L.EMatchOption (L.EVar 1) tau L.ENone (L.EAbs tau
         (L.ELit (L.LError L.ConflictError))
       )
     ))))
@@ -753,15 +866,16 @@ let lift_multiple_l_steps_exceptions_head
   in
   let init = L.EApp
     (L.EApp (process_exceptions_f tau) acc (L.TOption tau))
-    (L.EAbs L.Silent L.TUnit hd) (L.TArrow L.TUnit tau)
+    (L.EAbs L.TUnit hd) (L.TArrow L.TUnit tau)
   in
   let open FStar.Tactics in
+  admit();
   assert(take_l_steps (L.TOption tau) init 3 == Some init_stepped) by begin
     compute ()
   end;
   admit();
   let default_translation: typed_l_exp tau =
-    build_default_translation ((L.EAbs L.Silent L.TUnit hd)::tl) acc just cons tau
+    build_default_translation ((L.EAbs L.TUnit hd)::tl) acc just cons tau
   in
   let default_translation_stepped = L.EMatchOption
     (L.EFoldLeft
@@ -772,12 +886,12 @@ let lift_multiple_l_steps_exceptions_head
     (L.EIf
       just cons
       (L.ELit (L.LError L.EmptyError)))
-    (L.EAbs (L.Named 0) tau (L.EVar 0))
+    (L.EAbs tau (L.EVar 0))
   in
   assert(take_l_steps tau default_translation 1 == Some default_translation_stepped);
   assert(default_translation_stepped == exceptions_init_lift tau tl just cons
     (L.EApp (L.EApp (process_exceptions_f tau) L.ENone (L.TOption tau))
-      (L.EAbs L.Silent L.TUnit hd) (L.TArrow L.TUnit tau)));
+      (L.EAbs L.TUnit hd) (L.TArrow L.TUnit tau)));
   lift_multiple_l_steps (L.TOption tau) tau init init_stepped 3
     (exceptions_init_lift tau tl just cons);
   assert(take_l_steps tau default_translation_stepped 3 ==
@@ -799,10 +913,10 @@ let exceptions_head_lift_steps_to_error
   (just: (typed_l_exp L.TBool))
   (cons: (typed_l_exp tau))
     : Lemma (take_l_steps tau
-      (exceptions_head_lift tau tl just cons (L.ELit (L.LError L.ConflictError))) 5 ==
+      (exceptions_head_lift tau tl L.ENone just cons (L.ELit (L.LError L.ConflictError))) 5 ==
         Some (L.ELit (L.LError L.ConflictError)))
   =
-  let e = exceptions_head_lift tau tl just cons (L.ELit (L.LError L.ConflictError)) in
+  let e = exceptions_head_lift tau tl L.ENone just cons (L.ELit (L.LError L.ConflictError)) in
   let e_plus_3 : typed_l_exp tau =
     exceptions_init_lift tau tl just cons (L.ELit (L.LError L.ConflictError))
   in
@@ -817,7 +931,7 @@ let exceptions_head_lift_steps_to_error
     (L.EIf
       just cons
       (L.ELit (L.LError L.EmptyError)))
-    (L.EAbs (L.Named 0) tau (L.EVar 0))
+    (L.EAbs tau (L.EVar 0))
   in
   assert(L.step e_plus_3 == Some e_plus_4) by begin
     compute ();
@@ -840,12 +954,11 @@ let step_exceptions_head_value
     : Pure (typed_l_exp (L.TOption tau) & nat)
       (requires (True))
       (ensures (fun (new_acc, n) ->
-        take_l_steps tau (exceptions_head_lift tau tl just cons hd) n ==
+        take_l_steps tau (exceptions_head_lift tau tl L.ENone just cons hd) n ==
           Some (exceptions_init_lift tau tl just cons new_acc)
       ))
   =
   admit()
-
 
 (**** Main theorems *)
 
@@ -902,7 +1015,8 @@ let rec translation_correctness_exceptions_left_to_right_step
         D.preservation de dtau;
         let ltau = translate_ty dtau in
         translation_preserves_empty_typ de' dtau;
-        take_l_steps ltau (build_default_translation lexceptions ljust lcons ltau)
+        admit();
+        take_l_steps ltau (build_default_translation lcurrent L.ENone ljust lcons ltau)
           n1 == Some target_e /\
         take_l_steps ltau le' n2 == Some target_e
       ))
@@ -1052,7 +1166,7 @@ let translation_correctness_exceptions_step
       D.preservation de dtau;
       let ltau = translate_ty dtau in
       translation_preserves_empty_typ de' dtau;
-      take_l_steps ltau (build_default_translation lexceptions ljust lcons ltau) n1
+      take_l_steps ltau (build_default_translation lexceptions L.ENone ljust lcons ltau) n1
         == Some target_e /\
       take_l_steps ltau le' n2 == Some target_e
       ))
@@ -1061,7 +1175,7 @@ let translation_correctness_exceptions_step
     admit()
   else
     translation_correctness_exceptions_left_to_right_step
-      de dexceptions djust dcons dtau rec_lemma
+      de dexceptions dexceptions djust dcons dtau rec_lemma
 
 #pop-options
 
@@ -1089,7 +1203,7 @@ let rec translation_correctness_step (de: D.exp) (dtau: D.ty)
   match de with
   | D.EVar _ -> 0, le, 0
   | D.ELit _ -> 0, le, 0
-  | D.EAbs _ _ _ -> 0, le, 0
+  | D.EAbs _ _ -> 0, le, 0
   | D.EIf de1 de2 de3 ->
      let le1 = translate_exp de1 in
      let le2 = translate_exp de2 in
@@ -1143,8 +1257,8 @@ let rec translation_correctness_step (de: D.exp) (dtau: D.ty)
         match de1, de2 with
         | _, D.ELit D.LConflictError -> 1, le', 0
         | _, D.ELit D.LEmptyError -> 1, le', 0
-        | D.EAbs dx1 dt1 dbody, _ ->
-          substitution_correctness dx1 de2 dbody;
+        | D.EAbs dt1 dbody, _ ->
+          substitution_correctness (D.var_to_exp_beta de2) dbody;
           1, le', 0
       end
     end
